\documentclass[12pt]{article}
\usepackage[margin=1in]{geometry} 
\usepackage{amsthm}
\usepackage{amsmath}
\usepackage{amsfonts}
\usepackage{amssymb}
\usepackage{multicol}
\usepackage{graphicx}
\usepackage{float}
\usepackage{makecell}
\usepackage{fancyvrb} % size font inside verbatim environment
\newcommand{\verbatimfont}[1]{\renewcommand{\verbatim@font}{\ttfamily#1}}
\usepackage{siunitx}
\usepackage{blkarray} % show matrices with letters at borders
\usepackage{hyperref}
\usepackage{soul}
\usepackage{titling} % drop vertical space before the title
\sethlcolor{lightgray}
\setlength{\columnsep}{1cm}
\DeclareMathOperator{\R}{\mathbb{R}}
\renewcommand\qedsymbol{$\blacksquare$}

\setlength\parindent{0pt} %% Do not touch this

%% -----------------------------
%% TITLE
%% -----------------------------
\title{Problem Set 2} %% Assignment Title

\author{Jakub Gadawski\\ %% Student name
Optimization methods
}

\date{\today} %% Change "\today" by another date manually
%% -----------------------------
%% -----------------------------

%% %%%%%%%%%%%%%%%%%%%%%%%%%
\begin{document}
\setlength{\droptitle}{-5em}
%% %%%%%%%%%%%%%%%%%%%%%%%%%
\maketitle

% --------------------------
% Start here
% --------------------------

% %%%%%%%%%%%%%%%%%%%
\section*{Exercise 1}
% %%%%%%%%%%%%%%%%%%%
{\bfseries Check, if:}

% %%%%%%%%%%%%%%%%%%%
\subsection*{a) \( \forall_{i \in I} Z_i - convex \, set \implies \bigcap_{i \in I} Z_i - convex\,set\)}
\begin{proof}
    $ $\newline
    Let \(a,b \in \bigcap_{i \in I} Z_i\)\\
    We have to check, if \(\forall_{\lambda \in [0,1]} \lambda a + (1-\lambda)b \in \bigcap_{i \in I} Z_i\)\\
    But \( \forall_{i \in I} a, b \in Z_i\) and \(Z_i - convex\)\\
    Which means \(\forall_{i \in I} \forall_{\lambda \in [0,1]} \lambda a + (1-\lambda)b \in Z_i\)\\
    Which implies \(\forall_{\lambda \in [0,1]} \lambda a + (1-\lambda)b \in \bigcap_{i \in I} Z_i\)
\end{proof}


\subsection*{b) \( Z - convex\,set \implies conv(Z) = Z \)}
\begin{proof}
    $ $\newline
    Suppose, that \( Z - convex\,set \land conv(Z) \neq Z \)\\
    From definition of convex hull \(Z \subset conv(Z)\), so the only possibility to \(conv(Z) \neq Z\) is \(conv(Z) \nsubseteq Z\)\\
    From that \(\exists_{a,b \in Z}\exists_{\lambda\in [0,1]}: \lambda a + (1-\lambda)b \in conv(Z) \land \lambda a + (1-\lambda)b \notin Z \)\\
    But that implies, that \(Z - not\,convex\,set\), which goes against the assumption.
\end{proof}

\subsection*{c) \( Z_1, Z_2 - convex\,sets \implies Z_1+Z_2-convex\,set\)}
\begin{proof}
    $ $\newline
    Let \(x, y\in Z_1+Z_2\), that means \(\exists_{\substack{x_1, y_1 \in Z_1\\x_2,y_2 \in Z_2}}\quad x=x_1+x_2,\,y=y_1+y_2\) \\
    We have to check, if \(\forall_{\lambda \in [0,1]} \lambda x+(1-\lambda)y \in Z_1+Z_2\)\\
    Let's establish the specific \(\lambda \in [0,1]\)\\
    Consider points:
    \begin{center}
        \(\lambda x_1+(1-\lambda) y_1\ \in Z_1\) (because \(Z_1 - convex\,set\))\\
        \(\lambda x_2+(1-\lambda)y_2 \in Z_2\) (because \(Z_2 - convex\,set\))
    \end{center}
    Sum of that points: \(\lambda x_1+(1-\lambda) y_1 + \lambda x_2+(1-\lambda)y_2\)\\
    is producing \(\lambda (x_1+x_2)+(1-\lambda)(y_1+y_2)\),\\
    and that's \(\lambda x+(1-\lambda)y\)
\end{proof}
\newpage
\subsection*{d) \(Z_1 \subset \R^n, Z_2 \subset \R^m - convex\,sets \implies Z_1 \times Z_2 - convex\,set\,in\, \R^n \times \R^m\)}

\begin{proof}
    $ $\newline
    Let \(x, y \in Z_1 \times Z_2,\\
    x=(\overbrace{ a_1^1, a_2^1, \ldots, a_n^1}^{a_1}, \overbrace{ b_1^1, b_2^1, \ldots, b_m^1}^{b_1}),\,
    y=(\overbrace{ a_1^2, a_2^2, \ldots, a_n^2}^{a_2}, \overbrace{ b_1^2, b_2^2, \ldots, b_m^2}^{b_2})\\
    a_1,a_2 \in Z_1,\, b_1, b_2 \in Z_2 \)\\
    We have to check, if \(\forall_{\lambda \in [0,1]} \lambda x+(1-\lambda)y \in Z_1 \times Z_2\)\\
    We can rewrite it as \( \forall_{\lambda \in [0,1]}\\ (\lambda a^1_1+(1-\lambda)a^2_1, \lambda a^1_2+(1-\lambda)a^2_2, \ldots, \lambda a^1_n+(1-\lambda)a^2_n, \lambda b^1_1+(1-\lambda)b^2_1, \lambda b^1_2+(1-\lambda)b^2_2, \ldots, \lambda b^1_m+(1-\lambda)b^2_m ) \) \\
    Let's establish the specific \(\lambda \in [0,1]\)\\
    Consider points:
    \begin{center}
        \(\lambda a_1+(1-\lambda) a_2 \in Z_1\) (because \(Z_1 - convex\,set\))\\
        \(\lambda b_1+(1-\lambda)b_2 \in Z_2\) (because \(Z_2 - convex\,set\))
    \end{center}
    In Cartesian product \(Z_1 \times Z_2\) those points will give us:\\
    \((\lambda a^1_1+(1-\lambda)a^2_1, \lambda a^1_2+(1-\lambda)a^2_2, \ldots, \lambda a^1_n+(1-\lambda)a^2_n, \lambda b^1_1+(1-\lambda)b^2_1, \lambda b^1_2+(1-\lambda)b^2_2, \ldots, \lambda b^1_m+(1-\lambda)b^2_m ) \)\\
    and that's \(\lambda x+(1-\lambda)y \in Z_1 \times Z_2\)
\end{proof}

\subsection*{e) \( Z - convex\,set \implies \forall_{\alpha \in \R} \alpha Z - convex\,set\)}
\begin{proof}
    $ $\newline
    Let's establish specific \(\alpha \in \R\)\\
    Let \(x, y \in \alpha Z\)\\
    We have to check, if \(\forall_{\lambda \in [0,1]} \lambda x+(1-\lambda)y \in \alpha Z \)\\
    If \(x,y \in \alpha Z\), then \(\exists_{x_1, y_1 \in Z} x=\alpha x_1,\quad y=\alpha y_1\)\\
    Let's establish the specific \(\lambda \in [0,1]\)\\
    And consider point \(\lambda x+(1-\lambda)y\), equals \(\lambda \alpha x_1+(1-\lambda)\alpha y_1\)\\
    Let's transform to \(\alpha(\lambda  x_1+(1-\lambda) y_1)\)\\
    Point \(\lambda  x_1+(1-\lambda) y_1 \in Z\)
\end{proof}
\newpage
\section*{Exercise 2}
% %%%%%%%%%%%%%%%%%%%
{\bfseries Check, if sets are convex:}
\subsection*{a) \(H=\{x \in \R^n : <x,a> = \gamma \}, \quad a \in \R^n, \gamma \in \R\) }
Set H is the convex set
\begin{proof}
    $ $\newline
    Let \(x, y \in H\)\\
    We have to consider, if \(\forall_{\lambda \in [0,1]} \lambda x+(1-\lambda)y \in H\), or equivalently \( \forall_{\lambda \in [0,1]} <\lambda x+(1-\lambda)y, a>=\gamma\)\\
    \( <\lambda x+(1-\lambda)y, a>=<\lambda x, a>+<(1-\lambda)y, a>=\lambda<x, a>+(1-\lambda)<y, a> \)\\
    But we know (definition \(x, y\)), that \( <x, a> =\gamma,\quad <x, a> =\gamma\)\\
    Finally, we have \(\lambda\gamma+(1-\lambda)\gamma=\gamma \implies \lambda x+(1-\lambda)y \in H \)
\end{proof}
\subsection*{b) \(\R^n, \R^n_+\)}
Sets \(\R^n\) and \(\R^n_+\) are convex
\begin{proof}
    $ $\newline
    Let \(x, y \in \R^n,\quad x=(x_1, x_2, \ldots, x_n),\quad y=(y_1, y_2, \ldots, y_n), \quad \forall_{i \in \{1, \ldots, n \}}x_i, y_i \in \R\)\\
    Let's establish the specific \(\lambda\)\\
    Then, \( \lambda x+(1-\lambda)y = (\overbrace{\lambda x_1+(1-\lambda)y_1}^{\R},\overbrace{\lambda x_2+(1-\lambda)y_2}^{\R}, \ldots, \overbrace{\lambda x_n+(1-\lambda)y_n}^{\R}) \in \R^n\)\\
    $ $\newline
    Let \(x, y \in \R^n_+,\quad x=(x_1, x_2, \ldots, x_n),\quad y=(y_1, y_2, \ldots, y_n), \quad \forall_{i \in \{1, \ldots, n \}}x_i, y_i \in \R_+\)\\
    Let's establish the specific \(\lambda \in [0,1]\)\\
    Then, \( \lambda x+(1-\lambda)y = (\overbrace{\lambda x_1+(1-\lambda)y_1}^{\R_+},\overbrace{\lambda x_2+(1-\lambda)y_2}^{\R_+}, \ldots, \overbrace{\lambda x_n+(1-\lambda)y_n}^{\R_+}) \in \R^n_+\)\\
\end{proof}
\subsection*{c) Open/closed ball, sphere}
Open/closed ball is a convex set, sphere is not
\begin{proof}
    $ $\newline
    We can assume, that center of sphere/ball is \((0,0,0)\) and radius is equal \(r\) (We'll call it \(B\))\\
    Let \(x=(x_1, x_2, x_3),\quad y=(y_1, y_2, y_3),\quad x_1^2+x_2^2+x_3^2\leq r^2,\quad y_1^2+y_2^2+y_3^2\leq r^2\)\\
    Let's establish the specific \(\lambda \in [0,1]\)\\
    Then \(\lambda x+(1-\lambda)y=(\lambda x_1+(1-\lambda)y_1, \lambda x_2+(1-\lambda)y_2, \lambda x_3+(1-\lambda)y_3)\)\\
    We want to prove, that \( (\lambda x_1+(1-\lambda)y_1)^2+ (\lambda x_2+(1-\lambda)y_2)^2+ (\lambda x_3+(1-\lambda)y_3)^2\leq r^2 \)\\
    Let's transform left side of inequality to:\\ \( \lambda^2(\overbrace{x_1^2+x^2_2+x_3^2}^{\leq r^2})+2\lambda(1-\lambda)(\overbrace{x_1 y_1+x_2 y_2+x_3 y_3}^{We'll\,prove, \,that\,\leq r^2})+(1-\lambda)^2(\overbrace{y_1^2+y^2_2+y_3^2}^{\leq r^2})\leq \\ \leq r^2 (\lambda^2+2\lambda(1-\lambda)+(1-\lambda)^2) =r^2(\lambda+(1-\lambda))^2=r^2\)\\
    So, if only \(x_1 y_1+x_2 y_2+x_3 y_3\leq r^2,\,\lambda x+(1-\lambda)y \in B\)\\
    But, we can easily see, that:\\ \(x_1 y_1+x_2 y_2+x_3 y_3=<x, y>=\overbrace{|x|}^{\leq r}\overbrace{|y|}^{\leq r}\overbrace{\cos{\alpha}}^{\leq 1}\leq r^2 \quad\,\alpha \in [0,\pi]\)\\
    $ $\newline
    We can apply the same reasoning to open ball\\
    $ $\newline
    To sphere, let's take sphere with center in \((0,0,0)\) and radius 1. We can take segment \( S=((1, 0, 0), (-1, 0, 0))\). Then \((0,0,0) \in S\), but \((0,0,0)\) is not in sphere.
\end{proof}
\subsection*{d) \( E=\{ (x_1, x_2):3x_1^2+x_2^2 \geq 6 \}\)}
E is not a convex set
\begin{proof}
    $ $\newline
    Let's take points \(A=(-4,0), \, B=(4,0)\) and segment \(AB\)\\
    We can easily see, that \((0,0) \in AB\) and \( A, B \in E\), but \( (0,0)\notin E\)
\end{proof}
\subsection*{e) \( F=\{(x_1, x_2):x^1 x_2\leq 0 \land x_1, x_2\geq 0\}\)}
F is not a convex set
\begin{proof}
    $ $\newline
    Let's take points \(A=(0,2), \, B=(2,0)\) and segment \(AB\)\\
    We can easily see, that \((1,1) \in AB\) and \( A, B \in F\), but \( (0,0)\notin F\)
\end{proof}
\subsection*{f) \(Z=Z_1 \cup Z_2, Z_1, Z_2-convex\,sets\)}
Z is not a convex set
\begin{proof}
    $ $\newline
    Let's take sets \( Z_1=\{(x_1, x_2):x_1^2+x_2^2\leq 1, x_1, x_2 \in \R\}, Z_2=\{(3, 3)\} \)\\
    Then, \(Z=\{(x_1, x_2):x_1^2+x_2^2\leq 1\}\cup \{(2, 2)\}\)\\
    Because \(Z-convex\,set \implies \forall_{x, y \in Z} \forall_{\lambda \in [0,1]} \lambda x+(1-\lambda)y \in Z\)\\
    Let's take points \(A=(0,0), \, B=(3, 3)\) and segment \(AB\)\\
    We can easily see, that \((2,2) \in AB\) and \( A, B \in Z\), but \( (2,2)\notin Z\)
\end{proof}
\section*{Exercise 3}
{\bfseries Find convex hull of sets:}
\subsection*{a) \( Z=\{x, y\}, x \neq y, x,y \in \R^n\)}
For only two points, we have to take all points in segment \(xy\)\\
Then \(conv(Z) = \{ a:a=\lambda x + (1-\lambda)y, \lambda \in [0,1]\}\)
\subsection*{b) \( Z=\{x, y, z\}, x,y,z \in \R^n\, x, y, z - linearly\,intependent\)}
For three points, we have to take all points beetwen segments \(xy, yz, xz\)\\
Then \(conv(Z) = \{ a: a \in \bigtriangleup(xyz) \}\)
\subsection*{c) \( Z=\{(x_1, x_2) \in [0,1] \times [0,1]: x_1(x_1 - 1)=0 \land x_2(x_2 - 1)=0 \}\)}
We can consider set \(Z\) as set of four segments: \\ \( ((0,0), (0,1)), ((0,1), (1,1)), ((1,1), (1,0)), ((1,0), (0,0)) \)\\
Then \( conv(Z)= \{(x_1, x_2) \in [0,1] \times [0,1]: x_1(x_1 - 1) \leq 0 \land x_2(x_2 - 1) \leq 0 \}\)
\end{document}